\section*{Lecture 4}

\subsection*{1.}
Consider the system of equations
\begin{align*}
  x_2 + x_3 &= 2 \\
  2x_1 &= 1 \\
  2x_1 + x_2 + x_3 &= 3
.\end{align*}

\paragraph{a)} Solve the corresponding homogeneous system of equations.
\bigbreak
The corresponding homogeneous system of equations is
\begin{align*}
  x_{h2} + x_{h3} &= 0 \\
  2x_{h1} &= 0 \\
  2x_{h1} + x_{h2} + x_{h3} &= 0
.\end{align*}
This gives the augmented matrix
\[ 
\left( \begin{array}{ccc|c}
0 & 1 & 1 & 0\\
2 & 0 & 0 & 0\\
2 & 1 & 1 & 0\\
\end{array} \right)
.\]
We can now subtract (2) and (1) from (3) to get
\[ 
\left( \begin{array}{ccc|c}
0 & 1 & 1 & 0\\
2 & 0 & 0 & 0\\
0 & 0 & 0 & 0\\
\end{array} \right)
.\]
We can now exchange (1) and (2) to get
\[ 
\left( \begin{array}{ccc|c}
2 & 0 & 0 & 0\\
0 & 1 & 1 & 0\\
0 & 0 & 0 & 0\\
\end{array} \right)
.\]
This corresponds to the system of equations
\begin{align*}
  2x_{h1} &= 0 \\
  x_{h2} + x_{h3} &= 0
.\end{align*} 
The first equation implies that $x_{h1} = 0$ and from the second equation it becomes clear that an arbitrary constant $x_{h2} = c_2$ can be chosen which implies $x_{h3} = -c_2$. The solution is therefore
\[ 
\Vec{x}_h = \begin{pmatrix}
x_{h1}\\
x_{h2}\\
x_{h3}\\
\end{pmatrix} = \begin{pmatrix}
0\\
c_2\\
-c_2\\
\end{pmatrix} = c_2 \begin{pmatrix}
0\\
1\\
-1\\
\end{pmatrix}
.\]


\paragraph{b)} Find the general solution of the nonhomogeneous system of equations.
\bigbreak
We must first find one solution to the nonhomogeneous system of equations. We have the system
\begin{align*}
  x_{02} + x_{03} &= 2 \\
  2x_{01} &= 1 \\
  2x_{01} + x_{02} + x_{03} &= 3
.\end{align*}
We have the augmented matrix
\[ 
\left( \begin{array}{ccc|c}
0 & 1 & 1 & 2\\
2 & 0 & 0 & 1\\
2 & 0 & 0 & 3\\
\end{array} \right)
.\]
By subtracting (1) and (2) from (3) and switching around (1) and (2) we get
\[ 
\left( \begin{array}{ccc|c}
2 & 0 & 0 & 1\\
0 & 1 & 1 & 2\\
0 & 0 & 0 & 0\\
\end{array} \right)
.\]
This corresponds to the system of equations
\begin{align*}
  2x_{01} &= 1 \\
  x_{02} + x_{03} &= 2
.\end{align*}
From the first equation it is apparent that $x_{01} = \frac{1}{2}$ and in the second equation we can choose $x_{02} = 1 \implies x_{03} = 1$. We therefore have the solution
\[ 
\Vec{x}_0 = \begin{pmatrix}
x_{01}\\
x_{02}\\
x_{03}\\
\end{pmatrix} = \begin{pmatrix}
\frac{1}{2}\\
1\\
1\\
\end{pmatrix}
.\]
Therefore the general solution is
\[ 
\Vec{x} = \begin{pmatrix}
1 / 2\\
1\\
1\\
\end{pmatrix} + c_2 \begin{pmatrix}
0\\
1\\
-1\\
\end{pmatrix}
.\]



\subsection*{2.}
Consider the system of equations
\begin{align*}
  x_1 + x_2 + 2x_3 &= 1 \\
  2x_1 + 2x_2 &= 4\\
  x_1 + x_3 &= 2
.\end{align*}

\paragraph{a)} Solve the corresponding homogeneous system of equations.
\bigbreak
The corresponding homogeneous system of equations is
\begin{align*}
  x_1 + x_2 + 2x_3 &= 0 \\
  2x_1 + 2x_2 &= 0 \\
  x_1 + x_3 &= 0
.\end{align*}
The augmented matrix is
\[ 
\left( \begin{array}{ccc|c}
1 & 1 & 2 & 0\\
2 & 2 & 0 & 0\\
1 & 0 & 1 & 0\\
\end{array} \right)
.\]
We start by subtracting $2(1)$ from (2) to get
\[ 
\left( \begin{array}{ccc|c}
1 & 1 & 2 & 0\\
0 & 0 & -4 & 0\\
1 & 0 & 1 & 0\\
\end{array} \right)
.\]
We now subtract (1) from (3)
\[ 
\left( \begin{array}{ccc|c}
1 & 1 & 2 & 0\\
0 & 0 & -4 & 0\\
0 & -1 & -1 & 0\\
\end{array} \right)
.\]
We now exchange (2) and (3)
\[ 
\left( \begin{array}{ccc|c}
1 & 1 & 2 & 0\\
0 & -1 & -1 & 0\\
0 & 0 & -4 & 0\\
\end{array} \right)
.\]
The equivalent system of equations is
\begin{align*}
  x_{h1} + x_{h2} + 2x_{h3} &= 0 \\
  -x_{h2} - x_{h3} &= 0 \\
  -4x_{h3} &= 0
.\end{align*}
The third equation gives $x_{h3} = 0$, by inserting this into the second we get $x_{h2} = 0$ and by inserting these into the first we get $x_{h1} = 0$. This gives the solution
\[ 
\Vec{x}_h = \begin{pmatrix}
x_{h1}\\
x_{h2}\\
x_{h3}\\
\end{pmatrix} = \begin{pmatrix}
0\\
0\\
0\\
\end{pmatrix}
.\]



\paragraph{b)} Find the general solution of the nonhomogeneous system of equations.
\bigbreak
The nonhomogeneous system is
\begin{align*}
  x_{01} + x_{02} + 2x_{03} &= 1 \\
  2x_{01} + 2x_{02} &= 4 \\
  x_{01} + x_{03} &= 2
.\end{align*}
This gives the augmented matrix
\[ 
\left( \begin{array}{ccc|c}
1 & 1 & 2 & 1\\
2 & 2 & 0 & 4\\
1 & 0 & 1 & 2\\
\end{array} \right)
.\]
We subtract 2(1) from (2) to get
\[ 
\left( \begin{array}{ccc|c}
1 & 1 & 2 & 1\\
0 & 0 & -4 & 2\\
1 & 0 & 1 & 2\\
\end{array} \right)
.\]
We subtract (1) from (3) to get
\[ 
\left( \begin{array}{ccc|c}
1 & 1 & 2 & 1\\
0 & 0 & -4 & 2\\
0 & -1 & -1 & 1\\
\end{array} \right)
.\]
We exchange (2) and (3) to get
\[ 
\left( \begin{array}{ccc|c}
1 & 1 & 2 & 1\\
0 & -1 & -1 & 1\\
0 & 0 & -4 & 2\\
\end{array} \right)
.\]
This gives the equivalent system of equations
\begin{align*}
  x_{01} + x_{02} + 2x_{03} &= 1 \\
  -x_{02} - x_{03} &= 1 \\
  -4x_{03} &= 2
.\end{align*}
From the third equation we get $x_{03} = -\frac{1}{2}$, by inserting this into the second equation we get $x_{02} = -\frac{1}{2}$ and inserting these into the first equation we get $x_{01} = \frac{5}{2}$. This gives the single solution to the system of equations
\[ 
\Vec{x}_0 = \begin{pmatrix}
x_{01}\\
x_{02}\\
x_{03}\\
\end{pmatrix} = \begin{pmatrix}
5 / 2\\
-1 / 2\\
-1 / 2\\
\end{pmatrix}
.\]
Which gives the general solution
\[ 
\Vec{x}_0 = \begin{pmatrix}
5 / 2\\
-1 / 2\\
-1 / 2\\
\end{pmatrix} + \begin{pmatrix}
0\\
0\\
0\\
\end{pmatrix} = \begin{pmatrix}
5 / 2\\
- 1 / 2\\
- 1 / 2\\
\end{pmatrix}
.\]



\subsection*{3.}
Consider the system of equations
\[ 
A \Vec{x} = \Vec{b}, \quad A = \begin{pmatrix}
1 & 1 & 1 & 1\\
1 & 1 & 2 & 1\\
1 & 2 & 1 & 1\\
\end{pmatrix}, \quad \Vec{b} = \begin{pmatrix}
0\\
1\\
0\\
\end{pmatrix}
.\]

\paragraph{a)} Solve the corresponding homogeneous system of equations.
\bigbreak
The homogeneous system is $A \Vec{x}_h = 0$. This has the augmented matrix
\[ 
\left( \begin{array}{cccc|c}
1 & 1 & 1 & 1 & 0\\
1 & 1 & 2 & 1 & 0\\
1 & 2 & 1 & 1 & 0\\
\end{array} \right)
.\]
We subtract (1) from (2) and (3) to get
\[ 
\left( \begin{array}{cccc|c}
1 & 1 & 1 & 1 & 0\\
0 & 0 & 1 & 0 & 0\\
0 & 1 & 0 & 0 & 0\\
\end{array} \right)
.\]
We can now exchange (2) and (3) to get
\[ 
\left( \begin{array}{cccc|c}
1 & 1 & 1 & 1 & 0\\
0 & 1 & 0 & 0 & 0\\
0 & 0 & 1 & 0 & 0\\
\end{array} \right)
.\]
This corresponds to the system of equations
\begin{align*}
  x_{h1} + x_{h2} + x_{h3} + x_{h4} &= 0 \\
  x_{h2} &= 0 \\
  x_{h3} &= 0
.\end{align*}
We quickly observe that $x_{h2} = x_{h3} = 0$. By substituting this into the first equation we're left with
\[ 
  x_{h1} + x_{h4} = 0
.\]
If we choose an arbitrary value for $x_{h1} = c_1$ we get $x_{h4} = -c_1$. All in all this gives the solution
\[ 
\Vec{x}_h = \begin{pmatrix}
c_1\\
0\\
0\\
-c_1\\
\end{pmatrix} = c_1 \begin{pmatrix}
1\\
0\\
0\\
-1\\
\end{pmatrix}
.\]



\paragraph{b)} Find the general solution of the nonhomogeneous system of equations.
\bigbreak
We must first find one solution to the system of equations
\begin{align*}
  x_{01} + x_{02} + x_{03} + x_{04} &= 0 \\
  x_{01} + x_{02} + 2x_{03} + x_{04} &= 1 \\
  x_{01} + 2x_{02} + x_{03} + x_{04} &= 0
.\end{align*}
This corresponds to the augmented matrix
\[ 
\left( \begin{array}{cccc|c}
1 & 1 & 1 & 1 & 0\\
1 & 1 & 2 & 1 & 1\\
1 & 2 & 1 & 1 & 0\\
\end{array} \right)
.\]
We subtract (1) from (2) and (3) to get
\[ 
\left( \begin{array}{cccc|c}
1 & 1 & 1 & 1 & 0\\
0 & 0 & 1 & 0 & 1\\
0 & 1 & 0 & 0 & 0\\
\end{array} \right)
.\]
If we exchange (2) and (3) we get
\[ 
\left( \begin{array}{cccc|c}
1 & 1 & 1 & 1 & 0\\
0 & 1 & 0 & 0 & 0\\
0 & 0 & 1 & 0 & 1\\
\end{array} \right)
.\]
This gives the equivalent system of equations
\begin{align*}
  x_{01} + x_{02} + x_{03} + x_{04} &= 0 \\
  x_{02} &= 0 \\
  x_{03} &= 1
.\end{align*}
If we insert the bottom two equations into the first we get
\[ 
x_{01} + 0 + 1 + x_{04} = 0
.\]
If we choose $x_{01} = -1$ we get $x_{04} = 0$. This gives the single solution of
\[ 
\Vec{x}_0 = \begin{pmatrix}
x_{01}\\
x_{02}\\
x_{03}\\
x_{04}\\
\end{pmatrix} = \begin{pmatrix}
-1\\
0\\
1\\
0\\
\end{pmatrix}
.\]
The general solution is therefore
\[ 
\Vec{x} = \begin{pmatrix}
-1\\
0\\
1\\
0\\
\end{pmatrix} + c_1 \begin{pmatrix}
1\\
0\\
0\\
-1\\
\end{pmatrix}
.\]


\subsection*{4.}
Consider the system of equations
\[ 
A \Vec{x} = \Vec{b}, \quad A = \begin{pmatrix}
1 & 1 & 1 & 1\\
1 & 1 & 1 & 2\\
1 & 1 & 1 & 2\\
\end{pmatrix}, \quad \Vec{b} = \begin{pmatrix}
0\\
1\\
0\\
\end{pmatrix}
.\]

\paragraph{a)} Solve the corresponding homogeneous system of equations.
\bigbreak
We will first solve the homogeneous system of equations corresponding to $A \Vec{x}_h = \Vec{0}$. This gives the augmented matrix
\[ 
\left( \begin{array}{cccc|c}
1 & 1 & 1 & 1 & 0\\
1 & 1 & 1 & 2 & 0\\
1 & 1 & 1 & 2 & 0\\
\end{array} \right)
.\]
We can now subtract (2) from (3) to get
\[ 
\left( \begin{array}{cccc|c}
1 & 1 & 1 & 1 & 0\\
1 & 1 & 1 & 2 & 0\\
0 & 0 & 0 & 0 & 0\\
\end{array} \right)
.\]
Now we can subtract (1) from (2) to get
\[ 
\left( \begin{array}{cccc|c}
1 & 1 & 1 & 1 & 0\\
0 & 0 & 0 & 1 & 0\\
0 & 0 & 0 & 0 & 0\\
\end{array} \right)
.\]
This corresponds to the system of equations
\begin{align*}
  x_{h1} + x_{h2} + x_{h3} + x_{h4} &= 0 \\
  x_{h4} &= 0
.\end{align*}
By inserting the second equation into the first we get
\[ 
x_{h1} + x_{h2} + x_{h3} = 0
.\]
By choosing $x_{h2} = c_2$ and $x_{h3} = c_3$ we get $x_{h1} = -c_2 - c_3$. This gives the solution
\[ 
\Vec{x}_h = \begin{pmatrix}
x_{h1}\\
x_{h2}\\
x_{h3}\\
x_{h4}\\
\end{pmatrix} = \begin{pmatrix}
-c_2 - c_3\\
c_2\\
c_3\\
0\\
\end{pmatrix} = c_2 \begin{pmatrix}
-1\\
1\\
0\\
0\\
\end{pmatrix} + c_3 \begin{pmatrix}
-1\\
0\\
1\\
0\\
\end{pmatrix}
.\]



\paragraph{b)} Find the general solution of the nonhomogeneous system of equations.
\bigbreak
To find the general solution we must first find one solution. The last two equations, however, contradict each other and thus no general solution can be found.
