\section*{Lecture 2}

\subsection*{1)}
Consider the system of equations
\begin{align*}
  x_1 + 2x_2 + x_5 &= 0 \\
  x_2 + x_3 + x_4 &= 1 \\
  x_1 + x_4 + x_5 &= 2 \\
  x_2 + 3x_4 + x_5 &= 1 \\
  x_5 &= 1
.\end{align*}
Find the corresponding coefficient matrix $A$ and the corresponding augmented matrix $\tilde{A}$.
\bigbreak
We get the coefficient matrix $A$ as
\[ 
A = \begin{pmatrix}
1 & 2 & 0 & 0 & 1\\
0 & 1 & 1 & 1 & 0\\
1 & 0 & 0 & 1 & 1\\
0 & 1 & 0 & 3 & 1\\
0 & 0 & 0 & 0 & 1\\
\end{pmatrix}
.\]
And the augmented matrix $\tilde{A}$ as
\[ 
  \tilde{A} = \left( \begin{array}{ccccc|c}
  1 & 2 & 0 & 0 & 1 & 0\\
  0 & 1 & 1 & 1 & 0 & 1\\
  1 & 0 & 0 & 1 & 1 & 2\\
  0 & 1 & 0 & 3 & 1 & 1\\
  0 & 0 & 0 & 0 & 1 & 1\\
  \end{array} \right)
.\]



\subsection*{2)}
Consider the system of equations
\begin{align*}
  x_1 + x_2 + x_3 + 2x_5 &= 2 \\
  x_1 + 2x_2 + x_4 &= 1 \\
  2x_1 + x_4 + x_5 &= 2 \\
  x_2 + x_4 + x_5 &= 2
.\end{align*}
Find the corresponding coefficient matrix $A$ and the corresponding augmented matrix $\tilde{A}$.
\bigbreak
Once again $A$ is found as
\[ 
A = \begin{pmatrix}
1 & 1 & 1 & 0 & 2\\
1 & 2 & 0 & 1 & 0\\
2 & 0 & 0 & 1 & 1\\
0 & 1 & 0 & 1 & 1\\
\end{pmatrix}
.\]
And the augmented matrix is found as
\[ 
  \tilde{A} = \left( \begin{array}{ccccc|c}
  1 & 1 & 1 & 0 & 2 & 2\\
  1 & 2 & 0 & 1 & 0 & 1\\
  2 & 0 & 0 & 1 & 1 & 2\\
  0 & 1 & 0 & 1 & 1 & 2\\
  \end{array} \right)
.\]


\subsection*{3)}
Consider the system of equations
\begin{align*}
  x_1 + x_2 + 2x_3 &= 2 \\
  2x_1 + x_2 + x_3 &= 1 \\
  x_1 + x_4 + x_5 &= 2 \\
  x_1 + 2x_2 + x_3 &= 4 \\
  x_1 + x_2 &= 3 \\
  x_2 + x_4 &= 1
.\end{align*}
Find the corresponding coefficient matrix $A$ and the corresponding augmented matrix $\tilde{A}$.
\bigbreak
We have
\[ 
A = \begin{pmatrix}
1 & 1 & 2 & 0 & 0\\
2 & 1 & 1 & 0 & 0\\
1 & 0 & 0 & 1 & 1\\
1 & 2 & 1 & 0 & 0\\
1 & 1 & 0 & 0 & 0\\
0 & 1 & 0 & 1 & 0\\
\end{pmatrix}
.\]
And
\[ 
  \tilde{A} = \left( \begin{array}{ccccc|c}
  1 & 1 & 2 & 0 & 0 & 2\\
  2 & 1 & 1 & 0 & 0 & 1\\
  1 & 0 & 0 & 1 & 1 & 2\\
  1 & 2 & 1 & 0 & 0 & 4\\
  1 & 1 & 0 & 0 & 0 & 3\\
  0 & 1 & 0 & 1 & 0 & 1\\
  \end{array} \right)
.\]



\subsection*{4)}
Consider the augmented matrix
\[ 
  \tilde{A} =
\left( \begin{array}{cccc|c}
1 & 1 & 2 & 0 & 0\\
0 & 2 & 1 & 1 & 1\\
1 & 0 & 1 & 1 & 0\\
\end{array} \right)
.\]
Find the corresponding system of equations.
\bigbreak
We can apply the above method in reverse and get
\begin{align*}
x_1 + x_2 + 2x_3 &= 0 \\
2x_2 + x_3 + x_4 &= 1 \\
x_1 + x_3 + x_4 &= 0
.\end{align*}


\subsection*{5)}
Solve the system of equations
\begin{align*}
  x_1 + x_2 + x_3 &= 1\\
  x_1 + x_3 &= 1 \\
  x_2 + x_3 &= 1
.\end{align*}
\bigbreak
We can subtract (2) from (1) to get
\[ 
x_2 = 0
.\]
And we can quickly see that $x_2 = 0 \implies x_3 = 1, x_1 = 0$



\subsection*{6)}
Consider the matrix
\[ 
A = \begin{pmatrix}
1 & 1 & 1\\
2 & 1 & 2\\
0 & 1 & 1\\
\end{pmatrix}
.\]
Apply elementary row operations to transform it into the row equivalent matrix
\[ 
B = \begin{pmatrix}
1 & 0 & 0\\
0 & 1 & 0\\
0 & 0 & 1\\
\end{pmatrix}
.\]
\bigbreak
We start by subtracting (3) from (1) to get
\[ 
\begin{pmatrix}
1 & 0 & 0\\
2 & 1 & 2\\
0 & 1 & 1\\
\end{pmatrix}
.\]
We can now subtract $2(3)$ from (2) to get
\[ 
\begin{pmatrix}
1 & 0 & 0\\
2 & -1 & 0\\
0 & 1 & 1\\
\end{pmatrix}
.\]
Now $2(1)$ can be subtracted from (2)
\[ 
\begin{pmatrix}
1 & 0 & 0 \\
0 & -1 & 0\\
0 & 1 & 1 \\
\end{pmatrix}
.\]
(2) can be added to (3)
\[ 
\begin{pmatrix}
1 & 0 & 0\\
0 & -1 & 0\\
0 & 0 & 1\\
\end{pmatrix}
.\]
And (2) can be multiplied by $-1$
\[ 
\begin{pmatrix}
1 & 0 & 0\\
0 & 1 & 0\\
0 & 0 & 1\\
\end{pmatrix}
.\]



\subsection*{7)}
Consider the matrix
\[ 
A = \begin{pmatrix}
1 & 1 & 1\\
2 & 1 & 2\\
0 & 1 & 1\\
\end{pmatrix}
.\]
Apply elementary row operations to transform it to the row equivalent matrix
\[ 
B = \begin{pmatrix}
0 & 0 & 1\\
0 & 1 & 0\\
1 & 0 & 0\\
\end{pmatrix}
.\]
\bigbreak
Here we can start by applying all the same elementary row operations as before to get
\[ 
\begin{pmatrix}
1 & 0 & 0\\
0 & 1 & 0\\
0 & 0 & 1\\
\end{pmatrix}
.\]
And now we can apply the elementary row operation of switching equation between (1) and (3) to get
\[ 
\begin{pmatrix}
0 & 0 & 1\\
0 & 1 & 0\\
1 & 0 & 0\\
\end{pmatrix}
.\]
