\section*{Lecture 21}

\subsection*{1} Calculate the Laplace transform of
\[ 
f(t) = t \left( e^{t}-1 \right) 
.\]
\bigbreak
Here we use differentiation of Laplace transforms to get:
\begin{align*}
  F(s) &= \mathcal{L}\left( f(t) \right)  \\
  &= - \left( \mathcal{L}\left( e^{t}-1 \right)  \right)'  \\
  &= - \left( \frac{1}{s-1} - \frac{1}{s} \right)' \\
  &= - \left( - \frac{1}{\left( s-1 \right)^2} + \frac{1}{s^2} \right) \\
  &= \frac{1}{\left( s-1 \right)^2} - \frac{1}{s^2}
.\end{align*}


\subsection*{2.} Solve the IVP
\[ 
\Vec{y}'(t) = A \Vec{y}(t), \qquad A = \begin{pmatrix}
1 & -1\\
0 & 1\\
\end{pmatrix}, \qquad \Vec{y}(0) = \begin{pmatrix}
1\\
1\\
\end{pmatrix}
\]
using the Laplace transform.
\bigbreak
We start by writing the system as:
\begin{align*}
  y_1' &= y_{1}(t) - y_2(t) \\
  y_2' &= y_2(t)
.\end{align*}
This gives the system of subsidiaries:
\begin{align*}
  sY_1(s) - 1 &= Y_1(s) - Y_2(s) \\
  s Y_{2}(s) - 1 &= Y_2(s) \\
  \implies Y_1(s) &= \frac{1}{s-1} - \left( \frac{1}{s-1} \right)^2 \\
  Y_2(s) &= \frac{1}{s-1}
.\end{align*}
This gives the solutions:
\begin{align*}
  y_1(t) &= \mathcal{L}^{-1} \left( \frac{1}{s-1} \right) - \mathcal{L}^{-1} \left( \frac{1}{s-1} \frac{1}{s-1} \right)  \\
  &= e^{t} - \int_{0}^{t} e^{t - \tau} e^{t} \, \mathrm{d}\tau \\
  &= e^{t} - t e^{t}
.\end{align*}
And
\begin{align*}
  y_2(t) &= \mathcal{L}^{-1} \left( \frac{1}{s-1} \right) \\
         &= e^{t}
.\end{align*}



\subsection*{3.} Solve the IVP
\[ 
\Vec{y}''(t) = A \Vec{y}(t), \qquad A = \begin{pmatrix}
0 & 1\\
1 &0\\
\end{pmatrix}, \qquad \Vec{y}(0) = \begin{pmatrix}
-1\\
-1\\
\end{pmatrix}, \qquad \Vec{y}'(0) = \begin{pmatrix}
0\\
0\\
\end{pmatrix}
\]
using the Laplace transform.
\bigbreak
We write the system as:
\begin{align*}
  y_1''(t) &= y_2(t) \\
  y_2''(t) &= y_1(t)
.\end{align*}
Which gives the subsidiaries:
\begin{align*}
  s^2 Y_1(s) + s &= Y_2(s) \\
  s^2 Y_2(s) + s &= Y_1(s) \\
  \implies Y_1(s) &= - \frac{s}{s^2 - 1} \\
  Y_2(s) &= - \frac{s}{s^2 - 1}
.\end{align*}
Therefore the solutions are:
\begin{align*}
  y_1(t) &= \mathcal{L}^{-1} \left( - \frac{s}{s^2 - 1} \right) = - \cosh t \\
  y_2 (t) &= \mathcal{L}^{-1} \left( - \frac{s}{s^2 - 1} \right) = - \cosh t
.\end{align*}




\subsection*{4.} Solve the IVP
\[ 
\Vec{y}'(t) = A \Vec{y}(t) + \Vec{g}(t), \qquad A = \begin{pmatrix}
0 & 1\\
1 & 0\\
\end{pmatrix}, \qquad \Vec{y}(0) = \begin{pmatrix}
0\\
0\\
\end{pmatrix}, \qquad \Vec{g}(t) = \begin{pmatrix}
e^{t}\\
e^{t}\\
\end{pmatrix}
\]
using the Laplace transform.
\bigbreak
We start by writing the system as:
\begin{align*}
  y_1'(t) &= y_2(t) + e^{t} \\
  y_2'(t) &= y_1(t) + e^{t}
.\end{align*}
Which gives the subsidiaries:
\begin{align*}
  s Y_1(s) &= Y_2(s) + \frac{1}{s-1} \\
  s Y_2(s) &= Y_1(s) + \frac{1}{s-1}
.\end{align*}
Which has the solutions:
\begin{align*}
  Y_1(s) &= \frac{1}{\left( s-1 \right)^2} \\
  Y_2(s) &= \frac{1}{\left( s-1 \right)^2}
.\end{align*}
Which gives the solutions:
\begin{align*}
  y_1(t) &= \mathcal{L}^{-1} \left( \frac{1}{\left( s-1 \right)^2} \right)  \\
  &= \int_{0}^{t} e^{t - \tau} e^{\tau} \, \mathrm{d}\tau \\
  &= te^{t} \\
  y_2(t) &= \mathcal{L}^{-1}\left( \frac{1}{\left( s-1 \right)^2} \right) \\
         &= te^{t}
.\end{align*}
